src/coq/Utils/StateMonads.v
@@ -1,0 +1,33 @@
+From ExtLib Require Import
+     Structures.Monads
+     Structures.Functor.
+
+From ITree Require Import
+     ITree
+     Basics.Basics
+     Events.Exception
+     Eq.Eq
+     Events.StateFacts
+     Events.State.
+
+Import Basics.Basics.Monads.
+
+From Vellvm Require Import Utils.Monads.
+
+Import MonadNotation.
+
+(* TODO: move this? *)
+Definition runStateT {S M A} `{Monad M} (m: stateT S M A) (s : S) : M (A * S)%type
+  := '(s', a) <- m s;;
+     ret (a, s').
+
+Definition evalStateT {S M A} `{Monad M} (m: stateT S M A) (s : S) : M A
+  := fmap fst (runStateT m s).
+
+Global Instance MonadT_stateT_itree {S : Type} {M : Type -> Type} `{Monad M} : MonadT (stateT S M) M
+  := {| lift := fun (t : Type) (c : M t) => fun s => t0 <- c;; ret (s, t0) |}.
+
+Global Instance MonadState_stateT_itree {S : Type} {M : Type -> Type} `{Monad M} : MonadState S (stateT S M)
+  := {| MonadState.get := fun s => ret (s, s);
+        MonadState.put := fun x s => ret (x, tt);
+     |}.
