src/coq/Utils/UBAndErrors.v
@@ -1,0 +1,60 @@
+From Coq Require Import String.
+
+From ExtLib Require Import
+     Structures.Monads
+     Structures.MonadExc
+     Data.Monads.EitherMonad.
+
+From Vellvm.Utils Require Import Error.
+
+(* TODO: move these and use them in more places, so I'm less
+       confused by what string is which, e.g., in undef_or_err *)
+Inductive UB_MESSAGE :=
+| UB_message : string -> UB_MESSAGE
+.
+
+Inductive ERR_MESSAGE :=
+| ERR_message : string -> ERR_MESSAGE
+.
+
+Notation UB := (sum UB_MESSAGE).
+Notation ERR := (sum ERR_MESSAGE).
+
+Instance Exception_UB : MonadExc UB_MESSAGE UB := Exception_either UB_MESSAGE.
+Instance Exception_ERR : MonadExc ERR_MESSAGE ERR := Exception_either ERR_MESSAGE.
+
+Instance Exception_UB_string : MonadExc string UB :=
+  {| MonadExc.raise := fun _ msg => inl (UB_message msg);
+     catch := fun T c h =>
+                match c with
+                | inl (UB_message msg) => h msg
+                | inr _ => c
+                end
+  |}.
+
+Instance Exception_ERR_string : MonadExc string ERR :=
+  {| MonadExc.raise := fun _ msg => inl (ERR_message msg);
+     catch := fun T c h =>
+                match c with
+                | inl (ERR_message msg) => h msg
+                | inr _ => c
+                end
+  |}.
+
+Definition err_to_ERR {A} (e : err A) : ERR A
+  := match e with
+     | inl e => inl (ERR_message e)
+     | inr x => inr x
+     end.
+
+Definition lift_err {M A} `{MonadExc string M} `{Monad M} (e : err A) : (M A)
+  := match e with
+     | inl e => MonadExc.raise e
+     | inr x => ret x
+     end.
+
+Definition lift_ERR {M A} `{MonadExc ERR_MESSAGE M} `{Monad M} (e : ERR A) : (M A)
+  := match e with
+     | inl (ERR_message e) => MonadExc.raise (ERR_message e)
+     | inr x => ret x
+     end.
